KVOpenAddress.v: get_ok proof and most of a very messy put_ok proof that I should've committed weeks ago

src/KVOpenAddress.v
@@ -1,4 +1,3 @@
-Require Import Array.
 Require Import BasicProg.
 Require Import Hoare.
 Require Import FMapAVL.
@@ -12,6 +11,8 @@ Require Import Prog.
 Require Import SepAuto.
 Require Import Word.
 Require Import Omega.
+Require Import Permutation.
+Require Import Array.
 
 
 Module Map := FMapAVL.Make(Addr_as_OT).
@@ -27,6 +28,7 @@ Set Implicit Arguments.
 Parameter h: addr -> addr.
 Parameter maxlen : nat. (* Number of entries on disk *)
 Axiom hGood : forall a, # (h a) < maxlen.
+Axiom hEmpty : forall k, h empty_addr = h k -> False.
 
 Definition kvBase : addr := $0.
 
@@ -53,12 +55,120 @@ Fixpoint hash_rep l diskl : Prop :=
 
 Definition filter_empty l : (list entry) := filter (fun e => negb (beq_entry e empty_entry)) l.
 
+(*Inductive no_dup : (list entry) -> Prop :=
+  | ND_nil : no_dup nil
+  | ND_cons : forall l a,
+    no_dup l ->
+    ~In a l ->
+    no_dup (a :: l).*)
+
+Inductive no_dup : (list entry) -> Prop :=
+  | ND_nil : no_dup nil
+  | ND_cons : forall l key value,
+    no_dup l ->
+    ~In key (map fst l) ->
+     key <> empty_addr ->
+    no_dup ((key, value) :: l)
+  | ND_empty : forall l,
+    no_dup l ->
+    no_dup (empty_entry :: l).
+
+Lemma no_dup_updN :
+  forall diskl n default key value,
+    no_dup diskl ->
+    fst (selN diskl n default) = key ->
+    selN diskl n default <> empty_entry ->
+    no_dup (updN diskl n (key, value)).
+Proof.
+  induction diskl; intros.
+  auto.
+  destruct n; simpl in *; subst; inversion H.
+  constructor; auto.
+  simpl.
+  symmetry in H0. apply H1 in H0. inversion H0.
+  constructor; auto.
+  eapply IHdiskl; eauto.
+  rewrite map_updN. simpl.
+  rewrite <- map_updN. rewrite updN_selN_eq.
+  auto.
+  apply ND_empty.
+  eapply IHdiskl; auto.
+Qed.
+
+Lemma no_dup_upd:
+  forall diskl i default key value,
+    no_dup diskl ->
+    fst (sel diskl i default) = key ->
+    sel diskl i default <> empty_entry ->
+    no_dup (upd diskl i (key, value)).
+Proof.
+  intros. unfold sel, upd in *. eapply no_dup_updN; eauto.
+Qed.
+
+Lemma no_dup_selN :
+  forall diskl i j default,
+    no_dup diskl ->
+    i < length diskl ->
+    j < length diskl ->
+    selN diskl i default = selN diskl j default ->
+    selN diskl i default <> empty_entry ->
+    i = j.
+Proof.
+  induction diskl; intros.
+  inversion H0.
+  destruct i; destruct j; simpl in *; inversion H; auto.
+  - apply lt_S_n in H1.
+    eapply in_selN in H1.
+    assert (Ha: key = fst (selN diskl j default)).
+      rewrite <- H2. rewrite <- H4. auto.
+    rewrite Ha in H7.
+    eapply in_map in H1.
+    apply H7 in H1. inversion H1.
+  - intuition. symmetry in H4. apply H3 in H4. inversion H4.
+  - apply lt_S_n in H0.
+    eapply in_selN in H0.
+    assert (Ha: key = fst (selN diskl i default)).
+      rewrite H2. rewrite <- H4. auto.
+    rewrite Ha in H7.
+    eapply in_map in H0.
+    apply H7 in H0. inversion H0.
+  - intuition. subst. symmetry in H4. apply H3 in H4. inversion H4.
+  - replace i with j; auto.
+    eapply IHdiskl; eauto; try omega. rewrite <- H2. auto.
+  - replace i with j; auto.
+    eapply IHdiskl; eauto; try omega. rewrite <- H2. auto.
+Qed.
+
+Lemma no_dup_cons : forall diskl a,
+  no_dup (a :: diskl) ->
+  no_dup diskl.
+Proof.
+  induction diskl; simpl; intros; inversion H.
+  constructor. constructor.
+  destruct (beq_entry a a0) eqn:Heq.
+  - apply beq_entry_true in Heq.
+    subst.
+    auto.
+  - apply beq_entry_false in Heq.
+    inversion H2.
+    constructor.
+    eapply IHdiskl. eauto. auto. auto.
+    apply ND_empty; auto.
+  - auto.
+Qed.
+
+Definition hash_rep' l diskl := exists l',
+  hash_rep l diskl /\
+  filter_empty diskl = l' /\
+  Permutation l' l /\
+  no_dup diskl.
+
 Definition rep l := (exists diskl,
-  [[ hash_rep l diskl ]] *
+  [[ hash_rep' l diskl ]] *
   array kBase (map (fun e => addr2valu (fst e)) diskl) $2 *
   array vBase (map snd diskl) $2 *
-  [[ length diskl = maxlen ]] *
-  [[ filter_empty diskl = l ]])%pred.
+  [[ length diskl = maxlen ]]
+  )%pred.
 
 
 (* Is it enough to just be In the list? *)
@@ -101,7 +211,43 @@ Definition put T (key : addr) (value : valu) xp mscs rx : prog T :=
   }.
 
 
-Ltac solve_key_bound H := try (rewrite H; apply hGood).
+Fixpoint insert_l (l : list entry) (key : addr) (value : valu) : list entry :=
+  match l with
+  | nil => (key, value) :: nil
+  | (k, v) :: l' => if (weqb k key)
+                        then (k, value) :: insert_l l' key value
+                        else (k, v) :: insert_l l' key value
+  end.
+
+Definition insert_diskl
+  (diskl : list entry) (key : addr) (value : valu) : list entry :=
+  upd diskl (h key) (key, value).
+
+Lemma insert_diskl_length : forall diskl key value,
+  length (insert_diskl diskl key value) = length diskl.
+Proof.
+  intros.
+  unfold insert_diskl. rewrite length_upd. reflexivity.
+Qed.
+
+
+Lemma insert_diskl_filter_empty : forall l diskl key value,
+  Permutation l (filter_empty diskl) ->
+  Permutation (insert_l l key value) (filter_empty (insert_diskl diskl key value)).
+Proof.
+Admitted.
+
+Ltac solve_key_bound H :=
+  try rewrite map_length;
+  try rewrite insert_diskl_length;
+  try (rewrite H; apply hGood); auto.
+
+Ltac solve_diskl_equal :=
+  unfold insert_diskl;
+  try rewrite map_upd;
+  try rewrite skipn_upd;
+  try rewrite firstn_upd; auto.
+
 
 (* For any disk and key, if the key is on the disk, then the key and
     corresponding value are also in the current store (the non-empty entries
@@ -128,13 +274,14 @@ Proof.
   (* Shelved goal? *)
 Qed.
 
+
 (* For any (key, value) in the store, the key is stored at index h(key) on
     disk. *)
-Lemma hash_rep_key_index :
+Lemma hash_rep_index :
   forall l key value diskl,
     hash_rep l diskl ->
     In (key, value) l ->
-    key = fst (sel diskl (h key) empty_entry).
+    (key, value) = sel diskl (h key) empty_entry.
 Proof.
   intros l. induction l. intros. inversion H0.
   intros.
@@ -148,60 +295,655 @@ Proof.
 
   eapply IHl; auto.
   simpl in H.
-  (* How to get rid of let-binder in hypothesis? *)
   intuition.
   simpl in H0.
   apply beq_entry_false in aEq.
   intuition.
-  eauto.
+Qed.
+
+Lemma in_filter_empty_N:
+  forall diskl hkn,
+    empty_entry <> selN diskl hkn empty_entry ->
+    In (selN diskl hkn empty_entry) (filter_empty diskl).
+Proof.
+  induction diskl; simpl; intros.
+  - auto.
+  - destruct hkn.
+    + destruct (beq_entry a empty_entry) eqn:H'.
+      apply beq_entry_true in H'.
+      intuition.
+      symmetry in H'.
+      apply H in H'.
+      inversion H'.
+      simpl. intuition.
+    + destruct (negb (beq_entry a empty_entry)).
+      simpl.
+      right.
+      auto.
+      auto.
+Qed.
+
+Lemma in_filter_empty:
+  forall diskl hk,
+    empty_entry <> sel diskl hk empty_entry ->
+    In (sel diskl hk empty_entry) (filter_empty diskl).
+Proof.
+  unfold sel.
+  intros.
+  apply in_filter_empty_N.
+  auto.
+Qed.
+
+Lemma hash_rep'_well_formed_N :
+  forall diskl l hkn k v,
+    hash_rep' l diskl ->
+    selN diskl hkn empty_entry = (k, v) ->
+    (k, v) <> empty_entry ->
+    length diskl = maxlen ->
+    hkn < length diskl ->
+    hkn = # (h k).
+Proof.
+  unfold hash_rep'.
+  intros.
+  destruct H. intuition.
+  assert (In (selN diskl hkn empty_entry) l).
+    eapply Permutation_in. eauto.
+    rewrite <- H.
+    apply in_filter_empty_N.
+    congruence.
+
+  clear H H5.
+
+  induction l.
+  - inversion H6.
+  - inversion H4.
+    inversion H6.
+    + subst.
+      eapply no_dup_selN in H.
+      rewrite H0 in H. auto.
+      inversion H7.
+      constructor.
+      constructor; auto.
+      apply ND_empty. auto.
+      solve_key_bound H2. auto.
+      assert (Hd: selN diskl hkn empty_entry <> empty_entry).
+        intuition. apply H1. rewrite <- H0. auto.
+      unfold sel in H. rewrite H. auto.
+    + apply IHl; auto.
+Qed.
+
+Lemma hash_rep'_well_formed :
+  forall diskl l hk k v,
+    hash_rep' l diskl ->
+    sel diskl hk empty_entry = (k, v) ->
+    (k, v) <> empty_entry ->
+    length diskl = maxlen ->
+    # (hk) < length diskl ->
+    hk = h k.
+Proof.
+  intros.
+  rewrite <- natToWord_wordToNat.
+  erewrite <- hash_rep'_well_formed_N; eauto.
+  symmetry. apply natToWord_wordToNat.
 Qed.
 
 
-(* If the key is already in the store, ensure that it gets updated. *)
-Theorem put_ok1: forall key value xp mscs,
-  {< mbase MF l i,
-  PRE                   MEMLOG.rep xp MF (NoTransaction mbase) mscs *
-                        [[ (rep l)%pred (list2mem mbase) ]] *
-                        [[ key = selN (map fst l) i empty_addr ]]
-
-  POST RET:^(mscs', ok)
-                        ([[ ok = true ]] *
-                         exists m', MEMLOG.rep xp MF (NoTransaction m') mscs' *
-                         [[ (rep (updN l i (key, value)))%pred (list2mem m') ]]) \/
-                        ([[ ok = false ]] *
-                         MEMLOG.rep xp MF (NoTransaction mbase) mscs')
-
-  CRASH
-                        MEMLOG.would_recover_old xp MF mbase
-                        \/
-                        (exists m', MEMLOG.would_recover_either xp MF mbase m' *
-                         [[ (rep (updN l i (key, value)))%pred (list2mem m') ]])
-  >} put key value xp mscs.
+Lemma hash_rep_empty_index :
+  forall l key diskl,
+    hash_rep' l diskl ->
+    (forall key', h key = h key' -> forall v, ~In (key', v) l) ->
+    length diskl = maxlen ->
+    (*(~exists v, In (key, v) l) ->*)
+    empty_entry = sel diskl (h key) empty_entry.
 Proof.
-Admitted.
+  intros.
+  inversion H.
+  intuition.
 
-(* If the key is not already in the store, ensure that it gets inserted. *)
-Theorem put_ok2: forall key value xp mscs,
+  remember (sel diskl (h key) empty_entry) as foo.
+
+  destruct (beq_entry empty_entry foo) eqn:Hempty.
+  - apply beq_entry_true in Hempty.
+    auto.
+  - apply beq_entry_false in Hempty as HinL.
+    rewrite Heqfoo in HinL.
+    apply in_filter_empty in HinL.
+    assert (In foo l).
+      eapply Permutation_in. eauto. rewrite <- H2. rewrite Heqfoo. auto.
+    destruct foo as [k v].
+    exfalso.
+    eapply H0.
+      + apply beq_entry_false in Hempty.
+        eapply hash_rep'_well_formed; eauto.
+        solve_key_bound H1.
+      + eauto.
+Qed.
+
+Lemma hash_rep_empty_index' :
+  forall l key diskl,
+    hash_rep' l diskl ->
+    length diskl = maxlen ->
+    (*(~exists v, In (key, v) l) ->*)
+    empty_entry = sel diskl (h key) empty_entry ->
+    (forall key', h key = h key' -> forall v, ~In (key', v) l).
+Proof.
+  intros.
+  intuition.
+  unfold hash_rep' in H. inversion H. intuition.
+  eapply hash_rep_index in H5.
+  assert (Hempty: (key', v) <> empty_entry).
+    apply Permutation_in with (l':=x) in H3.
+    subst. unfold filter_empty in H3.
+    apply filter_In in H3.
+    inversion H3.
+    apply negb_true_iff in H7.
+    apply beq_entry_false in H7.
+    auto.
+  apply Permutation_sym. auto.
+  apply Hempty. rewrite H1. rewrite H2. rewrite <- H5. auto.
+  auto.
+Qed.
+
+Lemma hash_rep_empty_index'' :
+  forall l key diskl,
+    hash_rep' l diskl ->
+    length diskl = maxlen ->
+    (*(~exists v, In (key, v) l) ->*)
+    empty_entry = sel diskl (h key) empty_entry ->
+    key <> empty_addr ->
+    (forall key', key' <> empty_addr -> h key = h key' -> ~In key' (map fst diskl)).
+Proof.
+  intros. inversion H.
+  assert (Hl': ~In key' (map fst l)).
+    intuition.
+    apply in_map_iff in H6.
+    destruct H6. inversion H6.
+    eapply hash_rep_index with (value:=snd x0) in H7.
+    rewrite <- H4 in H7.
+    rewrite <- H1 in H7.
+    inversion H7. contradict H3. auto.
+    rewrite <- H9. rewrite <- surjective_pairing. auto.
+  intuition.
+  eapply Hl'.
+  eapply in_map_iff in H6.
+  destruct H6. inversion H6.
+  assert (Hfilter: In x0 diskl /\ (fun e => negb (beq_entry e empty_entry)) x0 = true).
+    split; auto.
+    apply negb_true_iff.
+    apply beq_entry_false_kv. left.
+    destruct x0. subst. auto.
+  eapply filter_In in Hfilter.
+  assert (Hfilter': In x0 (filter_empty diskl)). auto.
+  rewrite H5 in Hfilter'.
+  eapply Permutation_in in Hfilter'; eauto.
+  rewrite surjective_pairing with (p:=x0) in Hfilter'.
+  rewrite H9 in Hfilter'.
+  eapply hash_rep_empty_index' in H as Hl; eauto. instantiate (v:=snd x0).
+  apply Hl in Hfilter'. inversion Hfilter'.
+Qed.
+
+Lemma values_firstn_equal : forall l key value,
+  array vBase (firstn # (h key) (map snd l)) $ (2) =
+  array vBase (firstn # (h key) (map snd (insert_diskl l key value)))
+  $ (2).
+Proof.
+  intros. solve_diskl_equal.
+Qed.
+
+Lemma values_skipn_equal : forall l key value,
+array (vBase ^+ (h key ^+ $ (1)) ^* $ (2))
+  match map snd l with
+  | [] => []
+  | _ :: l0 => skipn # (h key) l0
+  end $ (2) =
+array (vBase ^+ (h key ^+ $ (1)) ^* $ (2))
+  match map snd (insert_diskl l key value) with
+  | [] => []
+  | _ :: l0 => skipn # (h key) l0
+  end $ (2).
+Proof.
+  intros. solve_diskl_equal.
+Qed.
+
+Lemma hkey_equal : forall l key value,
+  length l = maxlen ->
+  sel (insert_diskl l key value) (h key) (empty_entry) = (key, value).
+Proof.
+  intros. solve_diskl_equal.
+  eapply sel_upd_eq. solve_key_bound H.
+Qed.
+
+Lemma values_hkey_equal : forall l key value,
+  length l = maxlen ->
+  value = sel (map snd (insert_diskl l key value)) (h key) (empty_value).
+Proof.
+  intros.
+  erewrite sel_map.
+  rewrite hkey_equal; auto.
+  solve_key_bound H.
+Qed.
+
+Lemma keys_firstn_equal : forall l key value,
+  array kBase (firstn # (h key) (map (fun e : addr * valu => addr2valu (fst e)) l)) $ (2) =
+  array kBase
+    (firstn # (h key) (map (fun e : addr * valu => addr2valu (fst e)) (insert_diskl l key value)))
+    $ (2).
+Proof.
+  intros. solve_diskl_equal.
+Qed.
+
+Lemma keys_skipn_equal : forall l key value,
+  array (kBase ^+ (h key ^+ $ (1)) ^* $ (2))
+    match map (fun e : addr * valu => addr2valu (fst e)) l with
+    | [] => []
+    | _ :: l0 => skipn # (h key) l0
+    end $ (2) =
+  array (kBase ^+ (h key ^+ $ (1)) ^* $ (2))
+    match map (fun e : addr * valu => addr2valu (fst e)) (insert_diskl l key value) with
+    | [] => []
+    | _ :: l0 => skipn # (h key) l0
+    end $ (2).
+Proof.
+  intros. solve_diskl_equal.
+Qed.
+
+Lemma keys_hkey_equal : forall l key value,
+  length l = maxlen ->
+  addr2valu key = sel
+    (map (fun e : addr * valu => addr2valu (fst e))
+    (insert_diskl l key value)) (h key) (empty_value).
+Proof.
+  intros.
+  erewrite sel_map.
+  rewrite hkey_equal; auto.
+  solve_key_bound H.
+Qed.
+
+
+Lemma insert_hash_rep : forall l diskl key value,
+  length diskl = maxlen ->
+  hash_rep l diskl ->
+  fst (sel diskl (h key) empty_entry) = key ->
+  hash_rep (insert_l l key value) (insert_diskl diskl key value).
+Proof.
+  unfold insert_diskl. induction l; intros; simpl.
+  split; auto.
+  apply sel_upd_eq. solve_key_bound H.
+
+  destruct a as [k v].
+  destruct (weqb k key) eqn:kEq; simpl; split.
+  - rewrite weqb_true_iff in kEq.
+    rewrite kEq.
+    rewrite sel_upd_eq. auto. solve_key_bound H.
+  - simpl in H0. destruct H0.
+    apply IHl; auto.
+  - rewrite weqb_false_iff in kEq.
+    rewrite sel_upd_ne. symmetry.
+    eapply hash_rep_index.
+    + apply H0.
+    + simpl. auto.
+    + unfold not; intros. apply kEq.
+      rewrite <- H1. rewrite H2.
+      simpl in H0. destruct H0. rewrite H0. auto.
+  - simpl in H0. destruct H0.
+    apply IHl; auto.
+Qed.
+
+
+Lemma insert_hash_rep' : forall l diskl key value,
+  length diskl = maxlen ->
+  hash_rep' l diskl ->
+  fst (sel diskl (h key) empty_entry) = key ->
+  sel diskl (h key) empty_entry <> empty_entry ->
+  hash_rep' (insert_l l key value) (insert_diskl diskl key value).
+Proof.
+  unfold hash_rep'.
+  intros. inversion H0. intuition.
+  eexists.
+  intuition.
+  - apply insert_hash_rep; auto.
+  - apply Permutation_sym.
+    eapply insert_diskl_filter_empty.
+    apply Permutation_sym. congruence.
+  - unfold insert_diskl.
+    eapply no_dup_upd; eauto.
+Qed.
+
+
+Lemma no_dup_empty_updN : forall diskl key value n,
+  ~ In key (map fst diskl) ->
+  no_dup diskl ->
+  key <> empty_addr ->
+  no_dup (updN diskl n (key, value)).
+Proof.
+  induction diskl; intros.
+  constructor.
+  inversion H0.
+  - destruct n.
+    + simpl. constructor; auto. intuition.
+      apply H. simpl. right. auto.
+    + simpl. constructor.
+      * apply IHdiskl; auto.
+        intuition.
+        apply H. simpl. right. auto.
+      * intuition.
+        destruct (weqb key key0) eqn:Hkeykey0.
+        apply weqb_true_iff in Hkeykey0. subst.
+        apply H. simpl. auto.
+        apply H5.
+        apply weqb_false_iff in Hkeykey0.
+        contradict H5.
+        rewrite map_updN in H7. apply in_updN in H7.
+        destruct H7. auto.
+        simpl in H5. congruence.
+      * auto.
+  - destruct n.
+    + simpl. constructor; auto. intuition.
+      apply H. simpl. right. auto.
+    + simpl. apply ND_empty.
+      apply IHdiskl; auto.
+      intuition.
+      apply H. simpl. right. auto.
+Qed.
+
+Lemma insert_empty_no_dup : forall l diskl key value,
+  length diskl = maxlen ->
+  hash_rep' l diskl ->
+  sel diskl (h key) empty_entry = empty_entry ->
+  key <> empty_addr ->
+  no_dup (insert_diskl diskl key value).
+Proof.
+  intros l.
+  induction diskl; intros; inversion H0; intuition.
+  unfold insert_diskl, upd.
+  destruct # (h key) eqn:Hhkey.
+  - simpl.
+    inversion H7; try (
+      inversion H1;
+      unfold sel in H1; rewrite Hhkey in H1; simpl in H1;
+      subst; intuition;
+      constructor; auto;
+      eapply hash_rep_empty_index'' with (key:=key) in H0 as HIn; auto;
+      intuition;
+      apply HIn;
+      unfold In; simpl; right; apply H1).
+  - simpl. destruct a as [k v].
+    inversion H7.
+    destruct (weqb k key) eqn:HkeysEq.
+    + rewrite weqb_true_iff in HkeysEq. subst.
+      assert (Hcontra: (key, v) = sel ((key, v) :: diskl) (h key) empty_entry).
+          eapply hash_rep_index; eauto.
+        eapply Permutation_in in H5; eauto.
+        unfold filter_empty.
+        apply filter_In. split.
+        simpl. auto.
+        rewrite negb_true_iff.
+        apply beq_entry_false_kv. left. auto.
+      assert (HKey: (key, v) = empty_entry).
+        rewrite <- H1. auto.
+      inversion HKey. contradict H12. auto.
+    + subst. constructor.
+      eapply hash_rep_empty_index'' with (key:=key) in H0 as HIn; auto.
+      assert (HNoDupUpd: no_dup (updN diskl n (key, value))).
+        apply no_dup_empty_updN; auto.
+        intuition. apply HIn.
+        simpl. right. auto.
+      apply HNoDupUpd.
+      intuition. intuition. apply H11.
+      rewrite map_updN in H3. apply in_updN in H3.
+      inversion H3. auto.
+      apply weqb_false_iff in HkeysEq.
+      contradict HkeysEq. auto.
+      auto.
+    + apply ND_empty. apply no_dup_empty_updN; auto.
+      eapply hash_rep_empty_index'' with (key:=key) in H0; eauto.
+      intuition. apply H0.
+      simpl. right. auto.
+Qed.
+
+
+Lemma insert_empty_hash_rep : forall l diskl key value,
+  length diskl = maxlen ->
+  hash_rep l diskl ->
+  sel diskl (h key) empty_entry = empty_entry ->
+  key <> empty_addr ->
+  fst (selN l 0 empty_entry) <> key ->
+  h (fst (selN l 0 empty_entry)) <> h key ->
+  hash_rep (insert_l l key value) (insert_diskl diskl key value).
+Proof.
+  unfold insert_l, insert_diskl.
+  induction l; intros; simpl; intuition.
+  apply sel_upd_eq. solve_key_bound H.
+
+  destruct a as [k v].
+  destruct (weqb k key) eqn:HkEq; simpl.
+  + apply weqb_true_iff in HkEq.
+    contradict H3.
+    auto.
+  + apply weqb_false_iff in HkEq.
+    destruct (weqb (h k) (h key)) eqn:HhkEq; simpl.
+    - apply weqb_true_iff in HhkEq.
+      contradict H4.
+      auto.
+    - apply weqb_false_iff in HhkEq.
+      intuition.
+      replace (k, v) with (sel diskl (h k) empty_entry).
+      apply sel_upd_ne.
+      auto.
+      apply hash_rep_index with (key:=k) (value:=v) in H0.
+      auto.
+      simpl. auto.
+      inversion H0.
+      apply IHl; auto.
+      * intros.
+        apply hash_rep_index with (key:=key) (value:=snd (selN l 0 empty_entry)) in H6.
+        rewrite H1 in H6.
+        inversion H6.
+        apply H2 in H9. inversion H9.
+        rewrite <- H7.
+        rewrite <- surjective_pairing.
+        apply in_selN.
+        destruct l.
+          simpl in H7. symmetry in H7. apply H2 in H7. inversion H7.
+          simpl. omega.
+      * intros.
+        apply hash_rep_index with (key:=fst (selN l 0 empty_entry)) (value:=snd (selN l 0 empty_entry)) in H6.
+        rewrite H7 in H6.
+        rewrite H1 in H6.
+        inversion H6.
+        rewrite H9 in H7. apply hEmpty in H7. inversion H7.
+        rewrite <- surjective_pairing. apply in_selN.
+        destruct l. simpl in H7. apply hEmpty in H7. inversion H7.
+        simpl. omega.
+Qed.
+
+Lemma insert_empty_hash_rep' : forall l diskl key value,
+  length diskl = maxlen ->
+  hash_rep' l diskl ->
+  sel diskl (h key) empty_entry = empty_entry ->
+  key <> empty_addr ->
+  hash_rep (insert_l l key value) (insert_diskl diskl key value).
+Proof.
+  (* Prove
+      - ~In key l -> hash_rep (key, value) :: l diskl -> hash_rep (insert_l l (key, value)) diskl
+      - hash_rep l diskl -> sel diskl (h key) empty_entry = empty_entry -> ~In key l
+      - induction on l
+        prove every other element of l hashes to a different index from (h key) 
+        then insert_diskl updates some other index *)
+  induction l; intros. (*simpl; intuition.*)
+  unfold insert_l, insert_diskl.
+  simpl. intuition. apply sel_upd_eq. solve_key_bound H.
+
+  destruct a as [k v].
+  destruct (weqb k key) eqn:HkEq.
+  + unfold insert_l, insert_diskl.
+    simpl. apply weqb_true_iff in HkEq.
+    assert (Hcontra: ~In k (map fst diskl)).
+      eapply hash_rep_empty_index''; eauto.
+      rewrite HkEq. auto.
+    contradict Hcontra.
+    unfold hash_rep' in *.
+    inversion H0. intuition.
+    assert (HIn: In (k, v) x).
+      eapply Permutation_in.
+      apply Permutation_sym.
+      eauto.
+      simpl. auto.
+    apply in_map_iff. exists (k, v). intuition.
+    eapply filter_In.
+    rewrite <- H3 in HIn. unfold filter_empty in HIn.
+    eauto.
+  + apply weqb_false_iff in HkEq.
+    destruct (weqb (h k) (h key)) eqn:HhkEq.
+    - unfold insert_l, insert_diskl. apply weqb_true_iff in HhkEq.
+      unfold hash_rep' in *.
+      inversion H0.
+      inversion H3.
+      apply hash_rep_index with (key:=k) (value:=v) in H4.
+      rewrite HhkEq in H4.
+      rewrite H1 in H4.
+      inversion H5.
+      inversion H7. clear H0 H3 H5 H7.
+      assert (Hcontra: In empty_entry x).
+        eapply Permutation_in.
+        apply Permutation_sym. eauto.
+        rewrite H4. simpl. auto.
+      unfold filter_empty in *.
+      rewrite <- H6 in Hcontra.
+      apply filter_In in Hcontra.
+      inversion Hcontra.
+      apply negb_true_iff in H3.
+      unfold beq_entry in H3.
+      inversion H3.
+      apply weqb_false_iff in H7.
+      contradict H7. auto.
+      simpl. auto.
+    - apply weqb_false_iff in HhkEq.
+      unfold hash_rep' in *.
+      inversion H0.
+      intuition.
+      eapply insert_empty_hash_rep; auto.
+Qed.
+
+
+Lemma insert_empty_hash_rep'' : forall l diskl key value,
+  length diskl = maxlen ->
+  hash_rep' l diskl ->
+  sel diskl (h key) empty_entry = empty_entry ->
+  key <> empty_addr ->
+  hash_rep' (insert_l l key value) (insert_diskl diskl key value).
+Proof.
+  unfold hash_rep'.
+  intros.
+  eexists.
+  inversion H0.
+  intuition.
+  + apply insert_empty_hash_rep'; auto.
+  + symmetry.
+    apply insert_diskl_filter_empty.
+    symmetry. rewrite H3. auto.
+  + eapply insert_empty_no_dup; eauto.
+Qed.
+
+(* If the key is already in the store, ensure that it gets updated. *)
+Theorem put_ok: forall key value xp mscs,
   {< mbase MF l,
   PRE                   MEMLOG.rep xp MF (NoTransaction mbase) mscs *
                         [[ (rep l)%pred (list2mem mbase) ]] *
-                        [[ forall i, i < length l -> selN (map fst l) i empty_addr <> key ]]
+                        [[ length l < maxlen ]] *
+                        [[ key <> empty_addr ]]
 
   POST RET:^(mscs', ok)
                         ([[ ok = true ]] *
                          exists m', MEMLOG.rep xp MF (NoTransaction m') mscs' *
-                         [[ exists i, (rep (insN l i (key, value)))%pred (list2mem m') ]]) \/
+                         [[ (rep (insert_l l key value))%pred (list2mem m') ]]) \/
                         ([[ ok = false ]] *
                          MEMLOG.rep xp MF (NoTransaction mbase) mscs')
 
   CRASH
-                        MEMLOG.would_recover_old xp MF mbase
-                        \/
+                        MEMLOG.would_recover_old xp MF mbase \/
+                        MEMLOG.would_recover_either xp MF mbase mbase \/
                         (exists m', MEMLOG.would_recover_either xp MF mbase m' *
-                         [[ exists i, (rep (insN l i (key, value)))%pred (list2mem m') ]])
+                         [[ (rep (insert_l l key value))%pred (list2mem m') ]])
   >} put key value xp mscs.
 Proof.
+  unfold put. unfold rep.
+  step.
+  step.
+  rewrite isolate_fwd. cancel. unfold entry in *. solve_key_bound H8.
+  step.
+  step.
+  rewrite isolate_fwd with (a:=vBase). cancel. unfold entry in *. solve_key_bound H8.
+  step.
+  step.
+  apply pimpl_or_r. left. norm. cancel.
+  intuition.
+  exists (insert_diskl l key value).
+  pred_apply. cancel.
+  (* diskl array matches disk after insert *)
+  (*erewrite keys_equal. cancel.*)
+  rewrite <- isolate_bwd with (vs:=(map snd (insert_diskl l key value))).
+  cancel.
+  erewrite values_firstn_equal. erewrite values_skipn_equal. erewrite values_hkey_equal at 1.
+  cancel.
+  assert (Hkeys: array kBase (map (fun e : addr * valu => addr2valu (fst e)) (insert_diskl l key value)) $ (2) =
+                 array kBase (map (fun e : addr * valu => addr2valu (fst e)) l) $ (2)).
+    admit.
+  rewrite Hkeys. cancel.
+
+  auto.
+  solve_key_bound H8.
+  apply insert_hash_rep'; auto.
+  erewrite sel_map in H10.
+  apply addr2valu_inj in H10.
+  eauto.
+  admit. (* Why this bug? "solve_key_bound H7" should work *)
+  intuition.
+  rewrite sel_map with (default':=empty_entry) in H10.
+  apply addr2valu_inj in H10.
+  rewrite H in H10.
+  rewrite <- H10 in H4. contradict H4. auto.
+  solve_key_bound H8. solve_key_bound H8.
+
+  admit.
+  admit.
+
+  step.
+  step.
+  rewrite isolate_fwd. cancel. unfold entry in *. solve_key_bound H8.
+  step.
+  rewrite isolate_fwd with (a:=vBase). cancel. unfold entry in *. solve_key_bound H8.
+  step.
+  step.
+  apply pimpl_or_r. left. norm. cancel.
+  intuition.
+  exists (insert_diskl l key value).
+  pred_apply. cancel.
+  (* diskl array matches disk after insert *)
+  rewrite <- isolate_bwd with (vs:=(map snd (insert_diskl l key value))).
+  erewrite values_firstn_equal. erewrite values_skipn_equal. erewrite values_hkey_equal at 1.
+  cancel.
+  rewrite <- isolate_bwd with (vs:=(map (fun e : addr * valu => addr2valu (fst e)) (insert_diskl l key value))).
+  erewrite keys_firstn_equal. erewrite keys_skipn_equal. erewrite keys_hkey_equal. cancel.
+
+  auto.
+  solve_key_bound H8.
+  auto.
+  solve_key_bound H8.
+  apply insert_empty_hash_rep''; auto. admit.
+  solve_key_bound H9; assumption.
+
+  admit.
+  admit.
+
+  unfold MEMLOG.would_recover_old. cancel.
+  step.
+  step.
+  unfold MEMLOG.log_intact. cancel.
+
+  (* A bunch of MEMLOG things that I'm not sure about *)
 Admitted.
+
 
 Theorem get_ok: forall key xp mscs,
   {< mbase MF l,
@@ -222,9 +964,9 @@ Proof.
   step.
   step.
   (* h k = empty, key, or some other key k' where h k' = h k *)
-  rewrite isolate_fwd. cancel. rewrite map_length. unfold entry in *. rewrite H8. apply hGood.
+  rewrite isolate_fwd. cancel. rewrite map_length. unfold entry in *. solve_key_bound H9.
   step.
-  rewrite isolate_fwd with (a:=vBase). cancel. rewrite map_length. unfold entry in *. rewrite H8. apply hGood.
+  rewrite isolate_fwd with (a:=vBase). cancel. rewrite map_length. unfold entry in *. solve_key_bound H9.
 
   step.
   step.
@@ -241,7 +983,7 @@ Proof.
   intuition. apply H9. destruct H0.
   rewrite sel_map with (default':=empty_entry); solve_key_bound H8.
   replace (fst (l $[ h key])) with key; auto.
-  eapply hash_rep_key_index; eauto.
+  eapply hash_rep_index; eauto.
   unfold MEMLOG.would_recover_old. cancel.
   unfold MEMLOG.would_recover_old. cancel.
   unfold MEMLOG.would_recover_old. cancel.
